Using ST2 to compare the generated code to a manual projection

examples/relational/projection_tests/projection.fst
@@ -1,5 +1,5 @@
 (*--build-config
-    options:--admit_fsi FStar.Set --z3timeout 5 --project_module TEST --project_module TEST2 --project_module TEST3;
+    options:--admit_fsi FStar.Set --z3timeout 5;
     variables:LIB=../../../lib;
     other-files:$LIB/set.fsi $LIB/heap.fst $LIB/st.fst $LIB/all.fst $LIB/st2.fst 
   --*)
@@ -18,6 +18,6 @@ assume val r_PROJECT : #a:Type -> #b:Type -> a -> b
 assume type l_PROJECT_TYP: Type -> Type
 assume type r_PROJECT_TYP: Type -> Type
 
-type sem_equiv (t:Type) = unit -> ST2 (double t) 
-                                      (requires (fun h -> equal (R.l h) (R.r h)))
-                                      (ensures  (fun h1 r h2 -> (equal (R.l h2) (R.r h2)) /\ (R.l r) = (R.r r)))
+type sem_equiv (t:Type) = double unit -> ST2 (double t) 
+                                         (requires (fun h -> equal (R.l h) (R.r h)))
+                                         (ensures  (fun h1 r h2 -> (equal (R.l h2) (R.r h2)) /\ (R.l r) = (R.r r)))
