examples/relational/projection_tests/test_expected.fst
@@ -1,0 +1,78 @@
+(*--build-config
+    options:--admit_fsi FStar.Set --z3timeout 5 --project_module TEST --project_module TEST2 --project_module TEST3;
+    variables:LIB=../../../lib;
+    other-files:$LIB/set.fsi $LIB/heap.fst $LIB/st.fst $LIB/all.fst $LIB/st2.fst projection.fst TEST_projected.fst
+  --*)
+
+module TEST_exptected
+open TEST
+open Projection
+open FStar.Relational
+open FStar.Comp
+open FStar.Heap
+
+let r_expected = 0 
+
+val r_verify : sem_equiv int
+let r_verify tu = compose2 (fun () -> r) (fun () -> r_expected) tu
+
+let test_l_expected x = -x
+
+//val test_l_verify : int -> Tot (sem_equiv int)
+(* Unfolding because of #377 *)
+val test_l_verify : int -> 
+                    double unit -> ST2 (double int) 
+                                       (requires (fun h -> equal (R.l h) (R.r h)))
+                                       (ensures  (fun h1 r h2 -> (equal (R.l h2) (R.r h2)) /\ (R.l r) = (R.r r)))
+
+let test_l_verify x tu = compose2 (fun a -> test_l x) (fun a -> test_l_expected x) tu
+
+
+let test2_l_expected a b = a + b
+
+//val test2_l_verify : int -> int -> Tot (sem_equiv int)
+(* Unfolding because of #377 *)
+val test2_l_verify : int -> int ->
+                    double unit -> ST2 (double int) 
+                                       (requires (fun h -> equal (R.l h) (R.r h)))
+                                       (ensures  (fun h1 r h2 -> (equal (R.l h2) (R.r h2)) /\ (R.l r) = (R.r r)))
+
+let test2_l_verify a b tu = compose2 (fun x -> test2_l a b) (fun x -> test2_l_expected a b) tu
+
+
+let test3_l_expected a b c = (a + b) * c
+
+//val test3_l_verify : int -> int -> int -> Tot (sem_equiv int)
+(* Unfolding because of #377 *)
+val test3_l_verify : int -> int -> int ->
+                    double unit -> ST2 (double int) 
+                                       (requires (fun h -> equal (R.l h) (R.r h)))
+                                       (ensures  (fun h1 r h3 -> (equal (R.l h3) (R.r h3)) /\ (R.l r) = (R.r r)))
+
+let test3_l_verify a b c tu = compose2 (fun x -> test3_l a b c) (fun x -> test3_l_expected a b c) tu
+
+let test4_l_expected a b = 
+  match a + b with
+  | 0 -> 0
+  | 1 -> 1
+  | x -> x
+
+//val test4_l_verify : int -> int -> Tot (sem_equiv int)
+(* Unfolding because of #377 *)
+val test4_l_verify : int -> int -> 
+                    double unit -> ST2 (double int) 
+                                       (requires (fun h -> equal (R.l h) (R.r h)))
+                                       (ensures  (fun h1 r h4 -> (equal (R.l h4) (R.r h4)) /\ (R.l r) = (R.r r)))
+
+let test4_l_verify a b tu = compose2 (fun x -> test4_l a b) (fun x -> test4_l_expected a b) tu
+
+let test5_l_expected a b c = c := !a + !b
+
+//val test5_l_verify : ref int -> ref int -> ref int -> Tot (sem_equiv int)
+(* Unfolding because of #377 *)
+val test5_l_verify : a:ref int -> b:ref int{a <> b} -> c:ref int{c <> a /\ c <> b} -> 
+                    double unit -> ST2 (double unit) 
+                                       (requires (fun h -> equal (R.l h) (R.r h)))
+                                       (ensures  (fun h1 r h5 -> (equal (R.l h5) (R.r h5)) /\ (R.l r) = (R.r r)))
+
+let test5_l_verify a b c tu = compose2 (fun x -> test5_l a b c) (fun x -> test5_l_expected a b c) tu
